Express RecArray spec directly on vd
Eventually need to fix cache to hide readers for both the disk and
linear version of the disk, to make frames on both comparable.

src/ConcurrentRecArray.v
@@ -65,7 +65,7 @@ Module RecArray (Params:RecArrayParams).
   Lemma valu_wreclen_id : forall w, valu_to_wreclen (wreclen_to_valu w) = w.
   Proof.
     unfold valu_to_wreclen, wreclen_to_valu; intros.
-    eq_rect_simpl; auto.
+    now eq_rect_simpl.
   Qed.
 
   Lemma rep_valu_id : forall b, Rec.well_formed b -> valu_to_block (rep_block b) = b.
@@ -81,7 +81,7 @@ Module RecArray (Params:RecArrayParams).
   Proof.
     unfold valu_to_wreclen, wreclen_to_valu.
     intros.
-    eq_rect_simpl; auto.
+    now eq_rect_simpl.
   Qed.
 
   Lemma valu_rep_id : forall v,
@@ -92,15 +92,14 @@ Module RecArray (Params:RecArrayParams).
     apply wreclen_valu_id.
   Qed.
 
-  Tactic Notation "assert done" :=
-    let n := numgoals in guard n = 0.
-
   (* array_item_pairs *)
-  Definition rep_blocks (vs : list block) : @pred addr _ (const valu) :=
+  Definition rep_blocks (vs : list block) : @pred addr _ (const wr_set) :=
     ([[ length vs = RALen ]] *
      [[ Forall Rec.well_formed vs ]] *
-     array ($ RAStart) (map rep_block vs) $1)%pred.
+     (* TODO: eventually cache should not expose readers anywhere *)
+     array ($ RAStart) (map (fun b => (rep_block b, None)) vs) $1)%pred.
 
+  (* array_item *)
   Definition rep_items (vs : list item) :=
     (exists vs_nested, rep_blocks vs_nested *
                   [[ vs = concat vs_nested ]])%pred.
@@ -138,7 +137,7 @@ Module RecArray (Params:RecArrayParams).
       fun m s d =>
         ghost_lock_invariant (get Lock m) (get GLock s) /\
         (get GLock s = NoOwner -> get Items0 s = get Items s) /\
-        exists F, (get GDisk0 s |= F * rep_items (get Items0 s))%judgement.
+        exists F, (get GDisk s |= F * lin_point_pred (rep_items (get Items0 s)))%judgement.
 
   End RecArrayTransitions.
 
@@ -192,7 +191,7 @@ Module RecArray (Params:RecArrayParams).
     Import RATransitions.
 
     Definition rep (vs: list item) : type_pred Scontents :=
-      (exists l vs0, haddr GLock |-> l * haddr Items0 |-> vs0 * haddr Items |-> vs)%pred.
+      (exists l, haddr GLock |-> l * haddr Items |-> vs)%pred.
 
     Ltac derive_local :=
       match goal with
@@ -241,22 +240,29 @@ Module RecArray (Params:RecArrayParams).
 
     Polymorphic Theorem get_item_ok : forall i,
         stateS TID: tid |-
-        {{ Fs Fs' vs vd,
+        {{ Fs Fs' F LF F' vs vd,
          | PRE d m s0 s:
              hlistmem s |= Fs * rep vs * CacheM.rep vd /\
              Inv m s d /\
              get GLock s = Owned tid /\
              preserves' (fun s:S => hlistmem s) (star (othersR R tid)) Fs Fs'
                         (fun s => rep (get Items s) * CacheM.rep (get GDisk s))%pred /\
+             (forall P, preserves' (get GDisk) (star (othersR R tid))
+                              F F'
+                              (fun s => lin_latest_pred (cache_locked tid s P))) /\
+             vd |= F * lin_point_pred (rep_items vs) * lin_latest_pred (cache_locked tid s LF) /\
              R tid s0 s
          | POST d' m' s0' s' r:
-             exists vs' vd',
-               hlistmem s' |= Fs' * rep vs' * CacheM.rep vd' /\
+             exists vd',
+               hlistmem s' |= Fs' * rep vs * CacheM.rep vd' /\
                Inv m' s' d' /\
+               get GLock s' = Owned tid /\
+               vd' |= F' * lin_point_pred (rep_items vs) * lin_latest_pred (cache_locked tid s LF) /\
                r = selN vs i item0 /\
                R tid s0' s'
         }} get_item i.
     Proof.
+      hoare pre simplify with try solve [ finish ].
     Abort.
 
 
