src/ConcurrentCache2.v
@@ -449,18 +449,18 @@ Polymorphic Theorem locked_AsyncRead_ok : forall a,
        hlistmem s |= Fs * rep vd /\
        Inv m s d /\
        cache_get (get Cache m) a = None /\
-       vd |= F * lin_pred Latest
+       vd |= F * lin_latest_pred
         (cache_locked tid s (LF * a |-> (v, None))) /\
        preserves' (fun s:S => hlistmem s) (star (othersR R tid)) Fs Fs'
         (fun s => rep (get GDisk s))%pred /\
        (forall P, preserves' (get GDisk) (star (othersR R tid)) F F'
-        (fun s => lin_pred Latest (cache_locked tid s P))) /\
+        (fun s => lin_latest_pred (cache_locked tid s P))) /\
        R tid s0 s
    | POST d' m' s0' s' r:
        exists vd',
          hlistmem s' |= Fs' * rep vd' /\
          Inv m' s' d' /\
-         vd' |= F' * lin_pred Latest
+         vd' |= F' * lin_latest_pred
           (cache_locked tid s' (LF * a |-> (v, None))) /\
          r = v /\
          R tid s0' s'
@@ -590,17 +590,17 @@ Polymorphic Theorem locked_read_ok : forall a,
    | PRE d m s0 s:
        hlistmem s |= Fs * rep vd /\
        Inv m s d /\
-       vd |= F * lin_pred Latest (cache_locked tid s (LF * a |-> (v, None))) /\
+       vd |= F * lin_latest_pred (cache_locked tid s (LF * a |-> (v, None))) /\
        preserves' (fun s:S => hlistmem s) (star (othersR R tid)) Fs Fs'
         (fun s => rep (get GDisk s))%pred /\
        (forall P, preserves' (get GDisk) (star (othersR R tid)) F F'
-        (fun s => lin_pred Latest (cache_locked tid s P))) /\
+        (fun s => lin_latest_pred (cache_locked tid s P))) /\
        R tid s0 s
    | POST d' m' s0' s' r:
        exists vd',
          hlistmem s' |= Fs' * rep vd' /\
          Inv m' s' d' /\
-         vd' |= F' * lin_pred Latest (cache_locked tid s' (LF * a |-> (v, None))) /\
+         vd' |= F' * lin_latest_pred (cache_locked tid s' (LF * a |-> (v, None))) /\
          r = v /\
          R tid s0' s'
   }} read a.
@@ -661,17 +661,17 @@ Polymorphic Theorem locked_write_ok : forall a v,
      | PRE d m s0 s:
          hlistmem s |= Fs * rep vd /\
          Inv m s d /\
-         vd |= F * lin_pred Latest (cache_locked tid s (LF * a |-> (v0, None))) /\
+         vd |= F * lin_latest_pred (cache_locked tid s (LF * a |-> (v0, None))) /\
        preserves' (fun s:S => hlistmem s) (star (othersR R tid)) Fs Fs'
         (fun s => rep (get GDisk s))%pred /\
        (forall P, preserves' (get GDisk) (star (othersR R tid)) F F'
-        (fun s => lin_pred Latest (cache_locked tid s P))) /\
+        (fun s => lin_latest_pred (cache_locked tid s P))) /\
          R tid s0 s
      | POST d' m' s0' s' _:
          exists vd',
            hlistmem s' |= Fs' * rep vd' /\
            Inv m' s' d' /\
-           vd' |= F' * lin_pred Latest (cache_locked tid s' (LF * a |-> (v, None))) /\
+           vd' |= F' * lin_latest_pred (cache_locked tid s' (LF * a |-> (v, None))) /\
            R tid s0' s'
     }} write a v.
 Proof.
@@ -720,18 +720,18 @@ Polymorphic Theorem lock_ok : forall a,
      | PRE d m s0 s:
          hlistmem s |= Fs * rep vd /\
          Inv m s d /\
-         vd |= F * a |->? * lin_pred Latest (cache_locked tid s LF) /\
+         vd |= F * a |->? * lin_latest_pred (cache_locked tid s LF) /\
        preserves' (fun s:S => hlistmem s) (star (othersR R tid)) Fs Fs'
         (fun s => rep (get GDisk s))%pred /\
        (forall P, preserves' (get GDisk) (star (othersR R tid))
         (F * a |->?) (F' * a |->?)
-        (fun s => lin_pred Latest (cache_locked tid s P))) /\
+        (fun s => lin_latest_pred (cache_locked tid s P))) /\
          R tid s0 s
      | POST d' m' s0' s' _:
          exists vd' v,
            hlistmem s' |= Fs' * rep vd' /\
            Inv m' s' d' /\
-           vd' |= F' * lin_pred Latest (cache_locked tid s' (LF * a |-> (v, None))) /\
+           vd' |= F' * lin_latest_pred (cache_locked tid s' (LF * a |-> (v, None))) /\
            R tid s0' s'
     }} lock a.
 Proof.
@@ -825,7 +825,7 @@ Polymorphic Theorem unlock_ok : forall a,
      | PRE d m s0 s:
          hlistmem s |= Fs * haddr GDisk0 |-> vd0 * rep vd /\
          cacheI m s d /\
-         vd |= F * lin_pred Latest (cache_locked tid s (LF * a |-> (v, None))) /\
+         vd |= F * lin_latest_pred (cache_locked tid s (LF * a |-> (v, None))) /\
          vd0 |= F0 * a |-> v0 /\
          R tid s0 s
      | POST d' m' s0' s' _:
@@ -833,7 +833,7 @@ Polymorphic Theorem unlock_ok : forall a,
            hlistmem s' |= Fs * haddr GDisk0 |-> vd0' * rep vd' /\
            cacheI m' s' d' /\
            vd' |= F * a |-> ((v, None), (v, None)) *
-             lin_pred Latest (cache_locked tid s' LF) /\
+             lin_latest_pred (cache_locked tid s' LF) /\
            vd0' |= F0 * a |-> v /\
            s0' = s0
     }} unlock a.
